Refactor eventual guardedness of composition.

theories/OGS/CompGuarded.v
@@ -11,269 +11,201 @@ As described in §6.2, the proof relies crucially on the [eval_app_not_var] assu
 |*)
 
 From OGS Require Import Prelude.
-From OGS.Utils Require Import Ctx Rel.
+From OGS.Utils Require Import Psh Rel.
+From OGS.Ctx Require Import All Ctx.
 From OGS.OGS Require Import Subst Obs Machine Game Strategy.
 From OGS.ITree Require Import Event ITree Eq Delay Structure Properties Guarded.
 
-Open Scope ctx_scope.
+Require Import Coq.Arith.PeanoNat.
 
-Section withFam.
-
+Section with_param.
 (*|
-We consider a language abstractly captured as a machine
+We consider a language abstractly captured as a machine satisfying an
+appropriate axiomatization.
 |*)
-  Context {bT : baseT}.
-  Context {bV : baseV}.
-  Context {bC : baseC}.
-  Context {sV : subst_monoid bV}.
-  Context {sC : subst_module bV bC}.
-  Context {oS : observation_structure}.
-  Context {M: machine}.
-(*|
-Satisfying an appropriate axiomatization
-|*)
-  Context {sVL: subst_monoid_laws}.
-  Context {sCL: subst_module_laws}.
-  Context {VA : var_assumptions} .
-  Context {ML: machine_laws}.
+  Context `{CC : context T C} {CL : context_laws T C}.
+  Context {val} {VM : subst_monoid val} {VML : subst_monoid_laws val}.
+  Context {conf} {CM : subst_module val conf} {CML : subst_module_laws val conf}.
+  Context {obs : obs_struct T C} {M : machine val conf obs} {ML : machine_laws val conf obs}.
+  Context {VV : var_assumptions val}.
+
+  Notation ogs_ctx := (ogs_ctx (C:=C)).
 
 (*|
-A central elements in the proof lies in ensuring that there exists a unique solution to [compo_body]. Since the composition of strategies is defined as such a solution,
-adequacy can be established by proving that evaluating and observing the substituted term.
+A central elements in the proof lies in ensuring that there exists a unique solution
+to [compo_body]. Since the composition of strategies is defined as such a solution,
+adequacy can be established by proving that evaluating and observing the substituted
+term is also a solution of [compo_body].
 
 By [iter_evg_uniq], we know that eventually guarded equations admit a unique fixed point:
 we hence start by proving this eventual guardedness, captured in lemma [compo_body_guarded].
 |*)
 
-  Equations var_depth (Ψ : alt_ext) b {x} (j : ↓[b] Ψ ∋ x) : nat by struct Ψ :=
-    var_depth ∅%ctx        _     (!) ;
-    var_depth (Ψ ▶ Γ)%ctx true  i := aux Γ i
-      where aux (Γ1 : context) {x1} (i : (↓⁻ Ψ +▶ Γ1) ∋ x1) : nat by struct Γ1 := {
-        aux ∅%ctx         i1           := Datatypes.S (var_depth Ψ _ i1) ;
-        aux (Γ1 ▶ _)%ctx (Ctx.top)    := Datatypes.O ;
-        aux (Γ1 ▶ _)%ctx (Ctx.pop i1) := aux Γ1 i1
-      } ;
-    var_depth (Ψ ▶ Γ)%ctx false i := Datatypes.S (var_depth Ψ _ i).
-  Arguments var_depth {Ψ b x} j.
+  Equations var_height Φ p {x} : ↓[p]Φ ∋ x -> nat :=
+    var_height ∅ₓ       Pas i with c_view_emp i := { | ! } ;
+    var_height ∅ₓ       Act i with c_view_emp i := { | ! } ;
+    var_height (Φ ▶ₓ Γ) Pas i := var_height Φ Act i ;
+    var_height (Φ ▶ₓ Γ) Act i with c_view_cat i := {
+      | Vcat_l j := var_height Φ Pas j ;
+      | Vcat_r j := 1 + c_length Φ } .
+  #[global] Arguments var_height {Φ p x} i.
 
-  Lemma var_depth_ext {Ψ Γ x} (j : ↓⁻ Ψ ∋ x) :
-    @var_depth (Ψ ▶ Γ) true x (r_concat_l x j) = Datatypes.S (var_depth j) .
+  Lemma var_height_pos {Φ p x} (i : ↓[p]Φ ∋ x) : 0 < var_height i .
   Proof.
-    cbn.
-    pose (t' := r_concat_l (Δ:=Γ) x j); change (r_concat_l x j) with t' at 1.
-    pose (x' := x); change x with x' at 1; change x with x' in t'.
-    pose (Γ' := Γ); change Γ with Γ' at 1; change Γ with Γ' in t'.
-    remember t' as t_; clear Heqt_ t'.
-    remember x' as x_; clear Heqx_ x'.
-    remember Γ' as Γ_; clear HeqΓ_ Γ'.
-    revert x_ Γ_ t_; induction Γ; intros x_ Γ_ t_; cbn.
-    now rewrite r_cover_l_nil.
-    now apply IHΓ.
+    funelim (var_height i).
+    - apply H.
+    - rewrite <- Heqcall; apply H.
+    - rewrite <- Heqcall; apply Nat.lt_0_succ.
   Qed.
 
-  Definition var_height {Ψ : alt_ext} {b x} (j : ↓[b] Ψ ∋ x) : nat :=
-    Nat.sub (c_length Ψ) (var_depth j) .
+  Equations lt_bound : polarity -> relation nat :=
+    lt_bound Act := lt ;
+    lt_bound Pas := le .
 
-  Lemma var_depth_le {Ψ : alt_ext} {b x} (j : ↓[b] Ψ ∋ x) : (var_depth j <= c_length Ψ)%nat.
+  Lemma var_height_bound {Φ p x} (i : ↓[p]Φ ∋ x)
+    : lt_bound p (var_height i) (1 + c_length Φ).
   Proof.
-    revert b j; induction Ψ; intros b j; [ inversion j | ].
-    destruct b; cbn in *; [ | apply le_n_S, IHΨ ].
-    induction x0; [ apply le_n_S, IHΨ | ].
-    dependent elimination j; [ now apply le_0_n | now apply IHx0 ].
+    funelim (var_height i); cbn.
+    - now apply Nat.lt_succ_r, Nat.le_le_succ_r, Nat.le_le_succ_r.
+    - rewrite Heq; now apply Nat.lt_succ_r.
+    - rewrite Heq; apply Nat.lt_succ_diag_r.
   Qed.
 
-  Lemma depth_increases {Δ Ψ b} (v : alt_env Δ Δ b Ψ) {x} (j : ↓[negb b] Ψ ∋ x) (k : ↓[b] Ψ ∋ x)
-    (H : concat0 v x j = v_var x (r_concat_r x k)) : var_depth j < var_depth k.
+  Equations var_height' {Δ Φ p x} : Δ +▶ ↓[p]Φ ∋ x -> nat :=
+    var_height' i with c_view_cat i := {
+      | Vcat_l j := O ;
+      | Vcat_r j := var_height j } .
+
+  Lemma height_decrease {Δ Φ p} (v : ogs_env Δ p Φ) {x}
+        (j : ↓[p^] Φ ∋ x)
+        (H :  is_var (ₐ↓v _ j))
+        : var_height' (is_var_get H) < var_height j.
   Proof.
-    revert b v x j k H; induction Ψ; intros b v t j k H; [ inversion j | ].
-    destruct b; cbn in *.
-    - pose (k' := k); change k with k' at 1.
-      pose (x' := x); change x with x' at 1; change x with x' in k'.
-      pose (t' := t); change t with t' at 2; change t with t' in k'.
-      remember k' as k_; clear Heqk_ k'.
-      remember x' as x_; clear Heqx_ x'.
-      remember t' as t_; clear Heqt_ t'.
-      revert x_ t_ k_; induction x; intros x_ t_ k_.
-      * apply le_n_S.
-        (* dependent elimination v. *)
-        depelim v.
-        refine (IHΨ _ v _ j k _).
-        assert (H2 : @r_concat3_1 typ Δ ↓⁻ Ψ ∅ ≡ₐ r_id)
-          by (apply s_eq_cover_uniq; [ reflexivity | cbn; now rewrite r_cover_l_nil ]).
-        cbn in H; unfold e_ren in H.
-        unshelve erewrite (e_comp_proper _ v_var _ _ (concat0 v)) in H;
-          [ | now rewrite v_var_sub in H | reflexivity ].
-        etransitivity; [ apply s_ren_proper | apply s_ren_id ]; auto.
-      * depelim v; dependent elimination k; cbn in *.
-        (* dependent elimination v; dependent elimination k; cbn in *. *)
-      + pose (H' := (_ ,' H) : is_var _).
-        assert (Heq : is_var_get H' = Ctx.top) by reflexivity.
-        remember H' as H1; clear H' H HeqH1.
-        change ((?u ᵣ⊛ concat0 v) x1 j) with (u ᵣ⊛ᵥ concat0 v x1 j) in H1.
-        destruct (view_is_var_ren (concat0 v x1 j) _ H1); cbn in Heq.
-        destruct (cat_split (is_var_get p)).
-        ++ change (?u x1 _) with ((u ⊛ᵣ r_concat_l) _ i) in Heq.
-           unfold r_concat3_1 in Heq; rewrite s_eq_cat_l in Heq.
-           cbn in Heq; unfold s_ren, s_map, r_pop in Heq; inversion Heq.
-        ++ change (?u x1 _) with ((u ⊛ᵣ r_concat_r) _ j0) in Heq.
-           unfold r_concat3_1 in Heq; rewrite s_eq_cat_r in Heq.
-           cbn in Heq; unfold s_ren, s_map, r_pop in Heq; inversion Heq.
-      + apply (IHx (v ▶ₑ⁺) h); cbn.
-        pose (H' := (_ ,' H) : is_var _).
-        assert (Heq : is_var_get H' = (r_pop ⊛ᵣ r_cover_r cover_cat) x2 h) by reflexivity.
-        remember H' as H1; clear H' H HeqH1.
-        change ((?u ᵣ⊛ concat0 v) x2 j) with (u ᵣ⊛ᵥ concat0 v x2 j) in H1.
-        destruct (view_is_var_ren (concat0 v x2 j) _ H1).
-        destruct p; cbn in *.
-        unfold e_ren, e_comp, s_map; rewrite e, v_sub_id; unfold s_ren, s_map.
-        destruct (cat_split x0).
-        ++ change (r_concat3_1 x2 _) with ((@r_concat3_1 _ _ ↓⁻ Ψ (x ▶ y) ⊛ᵣ r_concat_l) x2 i) in Heq.
-           unfold r_concat3_1 in Heq; rewrite s_eq_cat_l in Heq.
-           change (r_concat3_1 x2 _) with ((@r_concat3_1 _ _ ↓⁻ Ψ x ⊛ᵣ r_concat_l) x2 i).
-           unfold r_concat3_1; rewrite s_eq_cat_l; unfold r_concat_l.
-           cbn in Heq; unfold r_pop, s_ren, s_map in Heq.
-           remember (@r_cover_l _ _ _ (Δ +▶ (↓⁻ Ψ +▶ x)) cover_cat x2 i).
-           remember (@r_cover_r _ _ _ (Δ +▶ (↓⁻ Ψ +▶ x)) cover_cat x2 h).
-           clear -Heq; now dependent induction Heq.
-        ++ change (r_concat3_1 x2 _) with ((@r_concat3_1 _ Δ _ (x ▶ y) ⊛ᵣ r_concat_r) x2 j0) in Heq.
-           unfold r_concat3_1 in Heq; rewrite s_eq_cat_r in Heq.
-           change (r_concat3_1 x2 _) with ((@r_concat3_1 _ Δ _ x ⊛ᵣ r_concat_r) x2 j0).
-           unfold r_concat3_1; rewrite s_eq_cat_r; unfold r_concat_l.
-           cbn in Heq; unfold r_pop, s_ren, s_map in Heq.
-           unfold s_ren, s_map, r_concat_r.
-           remember ((@r_cover_r _ _ _ (Δ +▶ (↓⁻ Ψ +▶ x)) cover_cat x2 (r_concat_l x2 j0))).
-           remember ((@r_cover_r _ _ _ (Δ +▶ (↓⁻ Ψ +▶ x)) cover_cat x2 (@r_cover_l _ _ _ (↓⁻ Ψ +▶ x) cover_cat x2 j0))).
-           clear -Heq; now dependent induction Heq.
-    - pose (j' := j); change j with j' at 1.
-      pose (x' := x); change x with x' at 1; change x with x' in j'.
-      pose (t' := t); change t with t' at 1; change t with t' in j'.
-      remember j' as j_; clear Heqj_ j'.
-      remember x' as x_; clear Heqx_ x'.
-      remember t' as t_; clear Heqt_ t'.
-      revert x_ t_ j_; induction x; intros x_ t_ j_.
-      * apply le_n_S.
-        depelim v.
-        (* dependent elimination v. *)
-        refine (IHΨ _ v _ j k _).
-        cbn in H; unfold s_cat, s_cover in H.
-        destruct (cover_split cover_cat j); [ | inversion j ].
-        cbn; rewrite r_cover_l_nil; exact H.
-      * dependent elimination j; [ apply PeanoNat.Nat.lt_0_succ | ].
-        depelim v; cbn.
-        (* dependent elimination v; cbn. *)
-        eapply (IHx (v ▶ₑ⁻ (a ⊛ᵣ r_pop))); cbn in *.
-        rewrite <- H.
-        change (([ ?u , a ]) x2 (pop h)) with (([ u , a ] ⊛ᵣ r_pop) x2 h).
-        apply s_eq_cover_uniq; rewrite <- s_ren_comp.
-      + change (r_pop ⊛ᵣ r_cover_l cover_cat) with (@r_cover_l _ _ _ (↓⁻ Ψ +▶ x ▶ y) cover_cat).
-        now rewrite s_eq_cat_l.
-      + change (r_pop ⊛ᵣ r_cover_r cover_cat) with (@r_cover_r _ _ _ (↓⁻ Ψ +▶ x ▶ y) cover_cat ⊛ᵣ r_pop).
-        now rewrite s_ren_comp, s_eq_cat_r.
+    revert H; rewrite lookup_collapse; intro H.
+    destruct (view_is_var_ren _ _ H).
+    rewrite ren_is_var_get; cbn.
+    remember (lookup v j).
+    destruct H; cbn; destruct (c_view_cat i).
+    - unfold var_height'; rewrite c_view_cat_simpl_l; apply var_height_pos.
+    - unfold var_height'; rewrite c_view_cat_simpl_r; cbn.
+      remember (r_ctx_dom j).
+      funelim (r_ctx_dom j); try clear Heqcall.
+      + cbn; rewrite c_view_cat_simpl_l; cbn.
+        dependent destruction v; now apply (H _ v).
+      + dependent destruction v.
+        revert j1 Heqv0; cbn; rewrite Heq; cbn; intros j1 Heqv.
+        now apply (H _ v).
+      + dependent destruction v; clear Heqv0.
+        revert j1; cbn; rewrite Heq; exact var_height_bound.
   Qed.
+
+  Definition compo_body_guarded_aux_stmt {Δ Φ} (u : ogs_env Δ Act Φ) (v : ogs_env Δ Pas Φ)
+    {x} (o : obs x) (γ : dom o =[val]> (Δ +▶ ↓⁺ Φ)) (j : ↓⁺ Φ ∋ x) : Prop
+    := ev_guarded
+         (fun 'T1_0 => compo_body)
+         (compo_body (RedT (MS ((ₐ↓v _ j ᵥ⊛ᵣ r_cat3_1) ⊙ o⦗r_cat_rr ᵣ⊛ a_id⦘)
+                               (v ;⁺))
+                           (u ;⁻ γ))) .
 
   Lemma compo_body_guarded_aux
-    {Δ Ψ} (u : alt_env Δ Δ Ⓟ Ψ) (v : alt_env Δ Δ Ⓞ Ψ)
-    {x} (o : obs x) (γ : dom o ⇒ᵥ (Δ +▶ ↓⁺ Ψ)) (j : ↓⁺ Ψ ∋ x) :
-    ev_guarded (fun 'T1_0 => compo_body (Δ := Δ))
-        (compo_body
-           ((Ψ ▶ dom o),' (app (r_concat3_1 ᵣ⊛ᵥ concat0 v x j) o ((v_var ⊛ᵣ r_concat_r) ⊛ᵣ r_concat_r), v ▶ₑ⁺, u ▶ₑ⁻ γ))) .
+    {Δ Φ} (u : ogs_env Δ Act Φ) (v : ogs_env Δ Pas Φ)
+    {x} (o : obs x) γ j : compo_body_guarded_aux_stmt u v o γ j .
   Proof.
-    pose (o' := (x ,' o)).
-    revert γ j.
-    change x with (projT1 o').
-    change o with (projT2 o').
-    remember o' as o''; clear o' o x Heqo''; rename o'' into o.
-    pose (wf := eval_app_not_var o).
+    (* setup wf induction on no-infinite-redex *)
+    revert Φ u v γ j.
+    pose (o' := (x ,' o)); change x with (projT1 o'); change o with (projT2 o').
+    generalize o'; clear x o o'; intro o.
+    pose (wf := eval_app_not_var o); induction wf.
+    destruct x as [ x o ]; cbn [ projT1 projT2 ] in *.
+    clear H; rename H0 into IHred; intros Φ u v γ j.
 
-    revert Ψ u v; induction wf; intros Ψ u v γ j.
-    destruct x as [ x m ]; cbn [projT1 projT2] in *.
-
+    (* setup wf induction on no-infinite var lookup *)
     pose (h := lt_wf (var_height j)); remember (var_height j) as n.
-    revert Ψ u v γ j Heqn; induction h; intros Ψ u v γ j Heqn.
+    revert Φ u v γ j Heqn; induction h.
+    clear H; rename x0 into n, H0 into IHvar; intros Φ u v γ j Heqn.
 
-    unfold ev_guarded; cbn -[cat_split].
+    (* case: is lookup a variable? *)
+    unfold compo_body_guarded_aux_stmt.
+    pose (vv := ₐ↓ v x j); fold vv.
+    destruct (is_var_dec vv).
 
-    pose (vv := @r_concat3_1 typ Δ ↓⁻ Ψ (@dom _ _ x m) ᵣ⊛ᵥ concat0 v x j).
-    change (r_concat3_1 ᵣ⊛ᵥ _) with vv; destruct (is_var_dec vv).
+    (* lookup is a var: either final or step on no-infinite var lookup *)
+    - rewrite (is_var_get_eq i); unfold vv in *; clear vv.
+      unfold v_ren; rewrite v_sub_var; unfold r_emb.
+      unfold ev_guarded; cbn.
 
-    - destruct i as [ i eq ].
-      rewrite eq.
-      eassert (H3 : _) by exact (eval_nf_ret (_ ,' (i , (m ,' ((v_var ⊛ᵣ r_concat_r) ⊛ᵣ r_concat_r))))).
-      unfold comp_eq in H3.
-      apply it_eq_step in H3; cbn in H3; unfold observe in H3.
-      pose (ot := _observe (eval (app (v_var x i) m ((v_var ⊛ᵣ r_concat_r) ⊛ᵣ r_concat_r)))); fold ot in H3 |- *.
-      destruct ot; dependent elimination H3.
-      cbn in r1, r_rel |- * .
-      destruct r1 as [ x' [ i' [ m' a' ] ] ].
-      destruct r_rel as [ p [ q r ] ]; cbn in *.
-      unfold m_strat_wrap; unfold obs' in a'; unfold obs'_of_nf', nf'_ty, nf'_var, nf'_obs in *; cbn [ fst snd projT1 projT2] in *.
-      revert i' m' a' q r; rewrite p; clear p x'; intros i' m' a' q [ r1 _ ]; cbn in q, r1.
-      rewrite q; clear q i'.
-      revert a'; rewrite r1; clear r1 m'; intros a'.
-      pose (i' := (i ,' eq) : is_var vv).
-      change i with (is_var_get i').
-      remember i' as ii; clear i i' Heqii eq.
-      unfold vv in ii; destruct (view_is_var_ren _ _ ii).
-      destruct p; simpl is_var_get.
-      destruct (cat_split x1).
-      * unfold r_concat3_1; change (?u x (r_cover_l _ x i)) with ((u ⊛ᵣ r_concat_l) x i).
-        rewrite s_eq_cat_l, cat_split_l.
-        now do 2 econstructor.
-      * unfold r_concat3_1; change (?u x (r_cover_r _ x j0)) with ((u ⊛ᵣ r_concat_r) x j0).
-        rewrite s_eq_cat_r; unfold s_ren, s_map; rewrite cat_split_r.
-        unfold obs'_dom, m_strat_resp; cbn [fst snd projT1 projT2].
-        refine (GNext _); eapply H2; [ | reflexivity ].
+      (* trickery to apply eval_nf_ret *)
+      pose proof (Heval :=
+                    eval_nf_ret ((r_cat3_1 x (is_var_get i)) ⋅ o ⦇ r_cat_rr ᵣ⊛ a_id  ⦈)).
+      unfold comp_eq in Heval; apply it_eq_step in Heval.
+      change (eval _) with
+        (eval (a_id (r_cat3_1 x (is_var_get i)) ⊙ o ⦗ r_cat_rr ᵣ⊛ a_id ⦘))
+        in Heval.
+      remember (eval (a_id (r_cat3_1 x (is_var_get i)) ⊙ o ⦗ r_cat_rr ᵣ⊛ a_id ⦘))
+        as tt; clear Heqtt.
+      remember (r_cat3_1 x (is_var_get i) ⋅ o ⦇ r_cat_rr ᵣ⊛ a_id ⦈) as ttn.
+      cbn in Heval; dependent destruction Heval.
+      rewrite Heqttn in r_rel; clear Heqttn.
+      dependent elimination r_rel.
+      unfold observe in x; rewrite <- x; clear x; cbn.
+      unfold m_strat_wrap, r_cat3_1; cbn.
+      remember (ₐ↓v _ j) as vv.
+      destruct i; cbn; destruct (c_view_cat i).
 
-        rewrite Heqn.
-        unfold var_height; rewrite var_depth_ext.
-        simpl c_length; rewrite PeanoNat.Nat.sub_succ.
-        apply (Plus.plus_lt_reg_l_stt _ _ (var_depth j0 + var_depth j)).
-        rewrite PeanoNat.Nat.add_shuffle0.
-        rewrite Arith_prebase.le_plus_minus_r_stt; [ | exact (@var_depth_le _ false _ j0) ].
-        rewrite <- PeanoNat.Nat.add_assoc.
-        rewrite Arith_prebase.le_plus_minus_r_stt; [ | exact (@var_depth_le Ψ _ _ j) ].
-        rewrite PeanoNat.Nat.add_comm.
-        apply Plus.plus_lt_compat_r_stt.
-        exact (depth_increases v j j0 e).
+      (* final channel, trivially guarded *)
+      + rewrite c_view_cat_simpl_l; now do 2 econstructor.
 
-    - remember (eval (app vv m ((v_var ⊛ᵣ r_concat_r) ⊛ᵣ r_concat_r))) as t.
-      remember (_observe t) as ot.
+      (* interaction, step on no-infinite var lookup *)
+      + rewrite c_view_cat_simpl_r; cbn.
+        refine (GNext _).
+        unshelve refine (IHvar _ _ _ _ _ _ _ eq_refl).
+        rewrite Heqn; clear Heqn; unfold cut_l.
+
+        (* trickery to apply height_decrease *)
+        clear tt ttn a1 a.
+        assert (i : is_var (ₐ↓v _ j)).
+          rewrite <- Heqvv.
+          now econstructor.
+        eapply Nat.lt_le_trans; [ | exact (height_decrease (p:=Pas) _ j i) ].
+        destruct i; cbn.
+        apply v_var_inj in Heqvv.
+        rewrite <- Heqvv; unfold var_height'.
+        rewrite c_view_cat_simpl_l, c_view_cat_simpl_r; cbn.
+        now apply Nat.lt_succ_diag_r.
+
+    (* lookup is not a var: step on no-infinite-redex *)
+    - unfold ev_guarded; cbn.
+      remember (eval ((vv ᵥ⊛ r_emb r_cat3_1) ⊙ o ⦗ r_cat_rr ᵣ⊛ a_id ⦘)) as tt.
+      remember (_observe tt) as ot.
       destruct ot; try now do 2 econstructor.
-      unfold m_strat_wrap.
-      destruct r as [ x' [ j' [ m' a' ]]]. unfold nf'_obs, nf'_val in *. cbn [ fst snd projT1 projT2 ].
-      pose (uu := cat_split j'); change (cat_split j') with uu; destruct uu.
-      now do 2 econstructor.
-      refine (GNext _).
-      unfold obs'_dom, obs'_obs; cbn [fst snd projT1 projT2].
-      eapply (H0 (x' ,' m')).
-      econstructor.
-      exact f.
+      destruct r as [ nx ni [ no narg ] ]; unfold m_strat_wrap; cbn.
+      destruct (c_view_cat ni); try now do 2 econstructor.
+      refine (GNext (IHred (_ ,' _) _ _ _ _ _ _)).
+
+      refine (HeadInst (_ ,' _) (vv ᵥ⊛ r_emb r_cat3_1) o
+                (r_cat_rr ᵣ⊛ a_id) (r_cat_r j0) (t ∘ (is_var_ren _ _)) _).
       apply it_eq_unstep; cbn.
-      rewrite Heqt in Heqot.
-      rewrite <- Heqot.
-      econstructor; reflexivity.
+      rewrite Heqtt in Heqot; rewrite <- Heqot.
+      now econstructor.
   Qed.
 
   Lemma compo_body_guarded {Δ} : eqn_ev_guarded (fun 'T1_0 => compo_body (Δ := Δ)).
   Proof.
-    intros [] [ Γ [ [c u] v ] ]; unfold m_strat_pas in v.
-    unfold ev_guarded; cbn -[cat_split].
+    intros [] [ Γ [ c u ] v ]; unfold m_strat_pas in v.
+    unfold ev_guarded; cbn.
     pose (ot := _observe (eval c)); change (_observe (eval c)) with ot.
     destruct ot; try now do 2 econstructor.
-    remember r as r'; rewrite Heqr'.
-    unfold m_strat_wrap; destruct r as [ ? [ i [ m γ ] ] ]; cbn in *.
-    destruct (cat_split i); try now do 2 econstructor.
-    refine (GNext _).
-    unfold obs'_dom, obs'_obs, obs'_ty; cbn [ fst snd projT1 projT2 ].
-    apply compo_body_guarded_aux.
+    destruct r as [ x i [ o a ] ]; unfold m_strat_wrap; cbn.
+    destruct (c_view_cat i); try now do 2 econstructor.
+    refine (GNext _); apply compo_body_guarded_aux.
   Qed.
 
-  Definition compo_ev_guarded {Δ a} (u : m_strat_act Δ a) (v : m_strat_pas Δ a) : delay (obs∙ Δ) :=
-    iter_ev_guarded _ compo_body_guarded T1_0 (a ,' (u , v)).
+  Definition compo_ev_guarded {Δ a} (u : m_strat_act Δ a) (v : m_strat_pas Δ a)
+    : delay (obs∙ Δ)
+    := iter_ev_guarded _ compo_body_guarded T1_0 (RedT u v).
 
-End withFam.
-
-Notation "u ∥g v" := (compo_ev_guarded u v) (at level 40).
+End with_param.
+#[global] Notation "u ∥g v" := (compo_ev_guarded u v) (at level 40).
 
 
 
